baseline done

theories/Main.v
@@ -1,5 +1,6 @@
 From Coq Require Import Nat.
 From Coq Require Import Arith. Import Nat.
+From Coq Require Import Datatypes.
 From Coq Require Import Lists.List.
 From Coq Require Import Program.Basics.
 From Coq Require Import Lia.
@@ -10,9 +11,50 @@ From Coq Require Import Extraction.
 From Coq Require Import ExtrHaskellBasic.
 From Coq Require Import ExtrHaskellNatNum.
 From Coq Require Import ExtrHaskellString.
-
+From Hask Require Import Data.Maybe.
+From Hask Require Import Data.Either.
+From Hask Require Import Data.Functor.
+From Hask Require Import Control.Applicative.
 
 Module Syntax.
+
+  Fixpoint digs (n : nat) (max : nat) {struct max} : list nat :=
+    match max with
+    | 0 =>
+        nil
+    | S max' =>
+        match n with
+        | 0 =>
+            nil
+        | n' =>
+            (modulo n' 10) :: digs (div n' 10) max'
+        end
+    end.
+
+  Fixpoint digs_to_string (ds : list nat) : string :=
+    match ds with
+    | nil =>
+        ""
+    | d :: ds' =>
+        (digs_to_string ds') ++
+        (String (ascii_of_nat (d + 48)) EmptyString)
+    end.
+
+  Definition nat_to_str (n : nat) : string :=
+    match n with
+    | 0 =>
+        "0"
+    | _ =>
+        digs_to_string (digs n 100)
+    end.
+
+  Definition bool_to_str (b : bool) : string :=
+    match b with
+    | true =>
+        "true"
+    | false =>
+        "false"
+    end.
 
   Inductive FExpr : Type :=
   | F_Var : string -> FExpr
@@ -27,15 +69,14 @@ Module Syntax.
     | E_Arith : AExpr -> Expr
 
   with BExpr : Type :=
-    | B_True : BExpr
-    | B_False : BExpr
+    | B_Const : bool -> BExpr
     | B_Not : BExpr -> BExpr
     | B_And : BExpr -> BExpr -> BExpr
     | B_Le : AExpr -> AExpr -> BExpr
+    | B_Func : FExpr -> BExpr
 
   with AExpr : Type :=
     | A_Const : nat -> AExpr
-    | A_Var : string -> AExpr
     | A_Add : AExpr -> AExpr -> AExpr
     | A_Sub : AExpr -> AExpr -> AExpr
     | A_Mult : AExpr -> AExpr -> AExpr
@@ -46,15 +87,7 @@ End Syntax.
 Module Semantics.
   Import Syntax.
 
-  Notation "f <$> m" := (option_map f m) (at level 50, left associativity).
-
-  Fixpoint ap {A B : Type} (f : option (A -> B)) (m : option A) : option B :=
-    match f with
-    | Some f' => f' <$> m
-    | None => None
-    end.
-
-  Notation "f <*> m" := (ap f m) (at level 50, left associativity).
+  Open Scope string_scope.
 
   Inductive Env : Type :=
   | EmptyEnv : Env
@@ -65,365 +98,198 @@ Module Semantics.
     | V_Closure : FExpr -> Env -> Value
     | V_ReturnValue : Value -> Value.
 
-
-  Example gpt : FExpr :=
-    F_Let "factorial" (F_Lambda "n"
-                    (F_Cond ((B_Le (A_Var "n") (A_Const 1)))
-                      (F_Return (E_Arith (A_Const 1)))
-                      (F_Return (E_Arith (A_Mult (A_Var "n") (A_Func (F_Apply (F_Var "factorial") (E_Arith (A_Sub (A_Var "n") (A_Const 1))))))))))
-      (F_Return (E_Arith (A_Func (F_Apply (F_Var "factorial") (E_Arith (A_Const 5)))))).
-
-
-  Fixpoint option_apply {A B : Type} (f : A -> option B) (x : option A) : option B :=
-    match x with
-    | Some x' => f x'
-    | None => None
-    end.
-
-  Inductive Either {A B : Type} : Type :=
-    | Right : B -> Either
-    | Left : A -> Either.
-
-  Definition either_map {A B C : Type} (f : A -> C) (either : Either) :=
-    match either with
-    | Right a => f a
-    | Left b => b
-    end.
-
-  Open Scope string_scope.
-
-  Fixpoint lookupEnv (env : Env) (varName : string) {struct env} : option Value :=
+  Fixpoint lookupEnv (varName : string) (env : Env) {struct env} : Maybe Value :=
     match env with
-    | EmptyEnv => None
+    | EmptyEnv => Nothing
     | ExtendEnv name value restEnv =>
         if String.eqb varName name
-        then Some value
-        else lookupEnv restEnv varName
+        then Just value
+        else lookupEnv varName restEnv
     end.
 
-  Fixpoint Feval (env : Env) (expr : FExpr) (max : nat) : @Either (list (string * option FExpr)) Value :=
+  Fixpoint env_to_string (env : Env) : string :=
+    match env with
+    | EmptyEnv => ""
+    | ExtendEnv name value restEnv =>
+        name ++ " = " ++ (value_to_string value) ++ ", " ++ (env_to_string restEnv)
+    end
+
+    with value_to_string (val : Value) : string :=
+      match val with
+      | V_Nat n => nat_to_str n
+      | V_Bool b => bool_to_str b
+      | V_Closure (F_Lambda paramName bodyExpr) closureEnv =>
+          "λ" ++ paramName ++ " -> " ++ ("[fexpr]") ++ ", " ++ (env_to_string closureEnv)
+      | V_ReturnValue v => "return " ++ (value_to_string v)
+      |   _ => "not impl"
+      end.
+
+  Fixpoint Feval (expr : FExpr) (env : Env) (max : nat) : Either (list (string * Maybe FExpr)) Value :=
     match max with
     | 0 =>
-        Left (("Error: Maximum recursion depth exceeded", None) :: nil)
+        Left (("Error: Maximum recursion depth exceeded", Nothing) :: nil)
     | S max' =>
       match expr with
       | F_Var varName =>
-          match lookupEnv env varName with
-          | Some value => Right value
-          | None =>
-              Left (("Error: Unbound variable", Some (F_Var varName)) :: nil)
+          match lookupEnv varName env with
+          | Just value =>
+              Right value
+          | Nothing =>
+              Left
+                (("(Feval) Error: Unbound variable"
+                 , Just (F_Var varName)) :: nil)
           end
       | F_Lambda paramName bodyExpr =>
           Right (V_Closure (F_Lambda paramName bodyExpr) env)
       | F_Apply funcExpr argExpr =>
-          match Feval env funcExpr max' with
-          | Right (V_Closure (F_Lambda paramName bodyExpr) closureEnv) =>
-              let argValueEither := Feval env (F_Return argExpr) max' in
+          match Feval funcExpr env max' with
+          | Right (V_Closure (F_Lambda paramName bodyExpr) _) =>
+              let argValueEither := Feval (F_Return argExpr) env max' in
               match argValueEither with
               | Right argValue =>
-                let extendedEnv := ExtendEnv paramName argValue closureEnv in
-                Feval extendedEnv bodyExpr max'
+                let extendedEnv := ExtendEnv paramName argValue env in
+                Feval bodyExpr extendedEnv max'
               | Left err =>
-                  Left 
-                    (("Error: Function argument did not evaluate to a value"
-                     , Some (F_Apply funcExpr argExpr)) :: nil)
+                  Left
+                    (("(Feval) Error: Function argument did not evaluate to a value"
+                     , Just (F_Apply funcExpr argExpr)) :: err)
               end
           | _ =>
               Left
-                (("Error: Attempted to apply a non-function"
-                 , Some (F_Apply funcExpr argExpr)) :: nil)
+                (("(Feval) Error: Attempted to apply a non-function"
+                 , Just (F_Apply funcExpr argExpr)) :: nil)
           end
       | F_Cond condExpr trueExpr falseExpr =>
           match Beval condExpr env max' with
-          | Some true =>
-              Feval env trueExpr max'
-          | Some false =>
-              Feval env falseExpr max'
-          | _ =>
-              Left
-                (("Error: Condition did not evaluate to a boolean"
-                 , Some (F_Cond condExpr trueExpr falseExpr)) :: nil)
+          | Right b =>
+              if b
+              then Feval trueExpr env max'
+              else Feval falseExpr env max'
+          | Left err =>
+              let newErr :=
+                ("(Feval) Error: Condition did not evaluate to a boolean"
+                 , Just (F_Cond condExpr trueExpr falseExpr))
+              in Left (newErr :: ((err , Nothing) :: nil))
           end
       | F_Let varName bindExpr bodyExpr =>
-          let bindValueEither := Feval env bindExpr max' in
+          let bindValueEither := Feval bindExpr env max' in
           match bindValueEither with
           | Right bindValue =>
             let extendedEnv := ExtendEnv varName bindValue env in
-            Feval extendedEnv bodyExpr max'
+            Feval bodyExpr extendedEnv max'
           | Left err =>
               Left
-                (("Error: Let binding did not evaluate to a value"
-                 , Some (F_Let varName bindExpr bodyExpr)) :: nil)
+                (("(Feval) Error: Let binding did not evaluate to a value"
+                 , Just (F_Let varName bindExpr bodyExpr)) :: err)
           end
       | F_Return retExpr =>
           match retExpr with
-          | E_Bool b => 
+          | E_Bool b =>
               match V_Bool <$> (Beval b env max') with
-              | Some v =>
+              | Right v =>
                   Right v
-              | None =>
+              | Left err =>
                   Left
-                    (("Error: Boolean expression did not evaluate to a boolean"
-                     , Some (F_Return retExpr)) :: nil)
+                    (("(Feval) Error: Boolean expression did not evaluate to a boolean"
+                     , Just (F_Return retExpr)) :: (err, Nothing) :: nil)
               end
           | E_Arith a =>
               match V_Nat <$> (Aeval a env max') with
-              | Some v =>
+              | Right v =>
                   Right v
-              | None =>
+              | Left err =>
                   Left
-                    (("Error: Arithmetic expression did not evaluate to a number"
-                     , Some (F_Return retExpr)) :: nil)
+                    (("(Feval) Error: Arithmetic expression did not evaluate to a number with env: "
+                        ++ env_to_string env
+                     , Just (F_Return retExpr)) :: (err, Nothing) :: nil)
               end
           end
       end
     end
 
-  with Aeval (a : AExpr) (env : Env) (max : nat) : option nat :=
+  with Aeval (a : AExpr) (env : Env) (max : nat) : Either string nat :=
     match max with
     | 0 =>
-        None
+        Left "(Aeval) Error: Maximum recursion depth exceeded"
     | S max' =>
       match a with
-      | A_Var n => 
-          match lookupEnv env n with
-          | Some (V_Nat n') =>
-              Some n'
-          | _ =>
-              None
-          end
       | A_Const n =>
-          Some n
+          Right n
       | A_Add a1 a2 =>
-          plus <$> (Aeval a1 env max') <*> (Aeval a2 env max')
+          add <$> (Aeval a1 env max') <*> (Aeval a2 env max')
       | A_Sub a1 a2 =>
           minus <$> (Aeval a1 env max') <*> (Aeval a2 env max')
       | A_Mult a1 a2 =>
           mult <$> (Aeval a1 env max') <*> (Aeval a2 env max')
-      | A_Func f => 
-          match Feval env f max' with
+      | A_Func f =>
+          match Feval f env max' with
           | Right (V_Nat n) =>
-              Some n
+              Right n
           | _ =>
-              None
+              Left
+                ("(Aeval) Error: Function did not evaluate to a number with env: "
+                 ++ env_to_string env)
           end
       end
     end
 
-  with Beval (b : BExpr) (e : Env) (max : nat) : option bool :=
+  with Beval (b : BExpr) (env : Env) (max : nat) : Either string bool :=
     match max with
     | 0 =>
-        None
+        Left "(Beval) Error: Maximum recursion depth exceeded"
     | S max' =>
       match b with
-      | B_True =>
-          Some true
-      | B_False =>
-          Some false
+      | B_Const b =>
+          Right b
       | B_Not b' =>
-          negb <$> Beval b' e max'
+          negb <$> Beval b' env max'
       | B_And b1 b2 =>
-          andb <$> (Beval b1 e max') <*> (Beval b2 e max')
+          andb <$> (Beval b1 env max') <*> (Beval b2 env max')
       | B_Le b1 b2 =>
-          Nat.leb <$> (Aeval b1 e max') <*> (Aeval b2 e max')
-      end
-    end.
-
-
-  Example bruh := F_Let "factorial" (F_Lambda "n"
-  (F_Cond
-    (B_Le (A_Var "n") (A_Const 1))
-    (F_Return (E_Arith (A_Const 1)))
-    (F_Return (E_Arith (A_Mult
-                (A_Var "n")
-                (A_Func (F_Apply (F_Var "factorial") (E_Arith (A_Sub (A_Var "n") (A_Const 1))))))))))
-  (F_Apply (F_Var "factorial") (E_Arith (A_Const 5))).
-
-  Example bruh2 :=
-    F_Return (E_Arith (A_Func (F_Return (E_Arith (A_Mult (A_Const 2) (A_Const 3)))))).
-
-  Compute Feval EmptyEnv bruh 100.
-  Compute Feval EmptyEnv bruh2 100.
-
-  Definition initialEnv : Env :=
-  ExtendEnv "n" (V_Nat 10)
-    (ExtendEnv "y" (V_Nat 5)
-      EmptyEnv).
- 
-  Definition initialEnv' : Env :=
-  ExtendEnv "factorial" (V_Closure
-                          (F_Lambda "n"
-                            (F_Cond
-                              (B_Le (A_Var "n") (A_Const 1))
-                              (F_Return (E_Arith (A_Const 1)))
-                              (F_Return
-                                (E_Arith 
-                                (A_Mult
-                                  (A_Var "n")
-                                  (A_Func 
-                                    (F_Apply
-                                      (F_Var "factorial")
-                                        (E_Arith
-                                          (A_Sub
-                                            (A_Var "n")
-                                            (A_Const 1)
-                                          )
-                                        )
-                                      )
-                                    )
-                                  ) 
-                                )
-                              )
-                            )
-                          )
-                        initialEnv)
-                        EmptyEnv.
-
-  Eval simpl in 
-    evalExpr
-    EmptyEnv
-    (F_Cond
-      (B_False)
-      (F_Return (E_Arith (A_Const 1)))
-      (F_Return (E_Arith (A_Const 2))))
-    1000.
-
-  Eval simpl in evalExpr initialEnv' bruh 1000.
-  Eval simpl in Feval bruh initialEnv' 1000.
-
-
-  Eval simpl in evalExpr initialEnv bruh 1000.
-
-  Inductive Ceval : CExpr -> State -> State -> Prop :=
-    | CE_Skip : forall s,
-        Ceval C_Skip s s
-    | CE_AssignA : forall s x e n,
-        Aeval e s = Some n ->
-        Ceval (C_AssignA x e) s (update_state_A s x (Some n))
-    | CE_AssignL : forall s x e n,
-        Leval e s = Some n ->
-        Ceval (C_AssignL x e) s (update_state_L s x (Some n))
-    | CE_Seq : forall c1 c2 s1 s2 s3,
-        Ceval c1 s1 s2 ->
-        Ceval c2 s2 s3 ->
-        Ceval (C_Seq c1 c2) s1 s3
-    | CE_IfTrue : forall b c1 c2 s1 s2,
-        Beval b s1 = Some true ->
-        Ceval c1 s1 s2 ->
-        Ceval (C_If b c1 c2) s1 s2
-    | CE_IfFalse : forall b c1 c2 s1 s2,
-        Beval b s1 = Some false ->
-        Ceval c2 s1 s2 ->
-        Ceval (C_If b c1 c2) s1 s2
-    | CE_WhileFalse : forall b c s,
-        Beval b s = Some false ->
-        Ceval (C_While b c) s s
-    | CE_WhileTrue : forall b c s1 s2 s3,
-        Beval b s1 = Some true ->
-        Ceval c s1 s2 ->
-        Ceval (C_While b c) s2 s3 ->
-        Ceval (C_While b c) s1 s3.
-
-
-  Fixpoint list_update_at_index (l : list nat) (n : nat) (v : nat) : list nat :=
-    match l with
-    | nil => nil
-    | cons x xs => match n with
-                   | O => cons v xs
-                   | S n' => cons x (list_update_at_index xs n' v)
-                   end
-    end.
-
-  Fixpoint Ceval_step (e : CExpr) (s : State) (max : nat) : State :=
-    match max with
-    | O => s
-    | S max' =>
-      match e with
-      | C_Skip => s
-      | C_AssignA x e =>
-          match Aeval e s with
-          | Some n => update_state_A s x (Some n)
-          | None => s
-          end
-      | C_AssignL x e =>
-          match Leval e s with
-          | Some n => update_state_L s x (Some n)
-          | None => s
-          end
-      | C_Seq c1 c2 => Ceval_step c2 (Ceval_step c1 s max') max'
-      | C_If b c1 c2 =>
-          match Beval b s with
-          | Some b' => if b' then Ceval_step c1 s max' else Ceval_step c2 s max'
-          | Nohting => s
-          end
-      | C_While b c =>
-          match Beval b s with
-          | Some b' => if b' then Ceval_step (C_Seq c (C_While b c)) s max' else s
-          | None => s
-          end
-      | C_Foreach x l c =>
-          match Leval l s with
-          | Some l' => 
-              fold_left (fun s' a => Ceval_step (C_Seq (C_AssignA x (A_Const a)) c) s' max') l' s
-          | None => s
-          end
-      | C_Print a => 
-          match Aeval a s with
-          | Some n => update_state_P s n
-          | None => s
-          end
-      | C_ListUpdate n i v =>
-          match Aeval i s, Aeval v s with
-          | Some i', Some v' => 
-              match L_State s n with
-              | Some l => update_state_L s n (Some (list_update_at_index l i' v'))
-              | None => s
-              end
-          | _, _ => s
+          Nat.leb <$> (Aeval b1 env max') <*> (Aeval b2 env max')
+      | B_Func f =>
+          match Feval f env max' with
+          | Right (V_Bool b) =>
+              Right b
+          | _ =>
+              Left
+               ("(Beval) Error: Function did not evaluate to a boolean with env: "
+                 ++ env_to_string env)
           end
       end
     end.
-
-  Open Scope string_scope.
-  Open Scope com_scope.
-
-  Definition swap :=
-    Ceval_step <{
-      "xs" @:= [1, 2, 3, 4, 5];
-      "ys" @:= [6, 7, 8, 9, 10];
-      "i" := 0;
-      "j" := 0;
-      foreach "x" in "xs" do
-        foreach "y" in "ys" do
-          if "x" < "y" then
-            "tmp" := "x";
-            (update "xs"["i"] to "y");
-            (update "ys"[A_Id "j"] to "tmp")
-          else
-            skip
-          end;
-          "j" := "j" + 1
-        done;
-        "i" := "i" + 1
-      done
-    }> empty_state 10000.
-
-  Compute A_State swap "i".
-  Compute A_State swap "j".
-  Compute L_State swap "xs".
-  Compute L_State swap "ys".
 
 End Semantics.
 
+Module Examples.
+
+  Import Syntax.
+  Import Semantics.
+
+  Example factorial :=
+    F_Let "factorial"
+      (F_Lambda "n"
+        (F_Cond
+          (B_Le (A_Func (F_Var "n")) (A_Const 1))
+          (F_Return (E_Arith (A_Const 1)))
+          (F_Return (E_Arith (A_Mult
+                      (A_Func (F_Var "n"))
+                      (A_Func (F_Apply (F_Var "factorial") (E_Arith (A_Sub (A_Func (F_Var "n")) (A_Const 1))))))))))
+      (F_Apply (F_Var "factorial") (E_Arith (A_Const 5))).
+
+  Example factorial_eval (n : nat) := Feval factorial EmptyEnv n.
+
+End Examples.
+
 Import Syntax.
 Import Semantics.
+Import Examples.
 
 Extraction Language Haskell.
 
-Extract Inductive option => "Prelude.Maybe" ["Prelude.Just" "Prelude.Nothing"].
 Extract Inductive nat => "Prelude.Integer" ["0" "Prelude.succ"]
   "(\fO fS n -> if n Prelude.== 0 then fO () else fS (n Prelude.- 1))".
-Extract Inlined Constant option_map => "(Prelude.<$>)".
-Extract Inlined Constant ap => "(Prelude.<*>)".
 
-Extraction "Haskell.hs" Ceval_step swap.
+Extraction
+  "Main.hs"
+  factorial_eval.
